src/Lib/DWT/Exec/Der_write_TL_m.v
@@ -1,18 +1,134 @@
 Require Import ExtLib.Structures.Monad Types.
 Require Import Core.Core Core.Notations Core.Tactics.
-Require Import Exec.Ber_tlv_tag_serialize_m
-        Exec.Ber_tlv_length_serialize_m.
+Require Import Exec.Ber_tlv_tag_serialize
+        Exec.Ber_tlv_length_serialize.
 Require Import VST.floyd.sublist.
 
 Open Scope Z.
 
+
+(* Definition der_write_TL tag len size constructed := 
+  let (tl, t) := tag_serialize tag (Int.repr size) in
+  let (ll, l) := length_serialize len (Int.repr (size - t)) in
+  let ls := if eq_dec constructed 0%int 
+            then tl ++ ll 
+            else (upd_Znth 0 tl (Znth 0 tl or (Int.repr 32))%int) ++ ll in
+  if ((t =? -1) || (32 <? t))%bool 
+  then ([], -1)
+  else if l =? -1 
+       then ([], -1) 
+       else let s := l + t in
+            if 32 <? s 
+            then ([], -1)
+            else (ls, s). *)
+
 Definition der_write_TL_m tag len size constructed : errW1 asn_enc_rval := 
  pass
- ('(encode t, tl) <- listen (tag_serialize tag (Int.repr size)) ;;
-  '(encode l, ll) <- listen (length_serialize len (Int.repr (size - t))) ;;
-  if (32 <? t) || (32 <? t + l) 
-  then raise (CustomError DWT_Error)
-  else if negb (constructed == 0%int) 
+   (let (tl, t) := tag_serialize tag (Int.repr size) in
+    let (ll, l) := length_serialize len (Int.repr (size - t)) in
+    if (32 <? t) || (32 <? t + l) 
+    then raise (CustomError DWT_Error)
+    else if negb (constructed == 0%int) 
        then ret (encode (t + l), id) 
-       else ret (encode (t + l), fun ls =>
+         else ret (encode (t + l), fun ls =>
                              (upd_Znth 0 ls (Znth 0 ls or (Int.repr 32))%int))).
+
+Lemma tag_serialize_bounds : forall t l, -1 <= snd (tag_serialize t l) <= 6.
+  { unfold tag_serialize.
+    intros.
+    cbn.
+    repeat break_if; autorewrite with norm; try nia. } 
+Qed.
+
+Lemma length_serialize_bounds : 
+  forall t l, -1 <= snd (length_serialize t l) <= 6.
+  { unfold length_serialize.
+    intros.
+    cbn.
+    repeat break_if; autorewrite with norm; try nia. } 
+Qed.
+
+(*Lemma tag_serialize_bounds :  forall t l z,
+    (evalErrW (tag_serialize t l)) [] = Some (encode z) -> 
+                               -1 <= z <= 6.
+Proof.
+ unfold tag_serialize.
+ intros.
+ repeat break_if; unfold evalErrW in *; cbn in *.
+ all: try congruence; repeat break_if; inversion H; 
+   try nia.
+Qed.
+
+
+Lemma length_serialize_bounds : forall t l z,
+    (evalErrW (length_serialize t l)) [] = Some (encode z) -> 
+                               -1 <= z <= 6.
+Proof.
+ unfold length_serialize.
+ intros.
+ repeat break_if; unfold evalErrW in *; cbn in *.
+ all: try congruence; repeat break_if; inversion H; 
+   try nia.
+Qed. *)
+
+(*
+
+Lemma der_write_TL_serialize_sum : 
+  forall t l s c, 
+    let (tls, tl) := tag_serialize t (Int.repr s)  in
+    let (lls, ll) := length_serialize l (Int.repr (s - tl)) in
+    tl <> -1 ->
+    ll <> -1 ->
+    tl <= 32 ->
+    tl + ll <= 32 ->
+    c = 0%int ->
+    der_write_TL t l s c = (tls ++ lls, tl + ll).
+Proof.
+  intros.
+  repeat break_let.
+  unfold der_write_TL.
+  intros Z Z0 Z32 Zplus C.
+  erewrite Heqp.
+  erewrite Heqp0.
+  repeat break_if; try destruct_orb_hyp;
+  repeat Zbool_to_Prop; try nia.
+  intuition.
+  congruence.
+Qed.
+
+Lemma der_write_TL_serialize_sum_c : 
+  forall t l s c, 
+    let (tls, tl) := tag_serialize t (Int.repr s)  in
+    let (lls, ll) := length_serialize l (Int.repr (s - tl)) in
+    tl <> -1 ->
+    ll <> -1 ->
+    tl <= 32 ->
+    tl + ll <= 32 ->
+    c <> 0%int ->
+    der_write_TL t l s c = ((upd_Znth 0 tls (Znth 0 tls or (Int.repr 32))%int) ++ lls, tl + ll).
+Proof.
+  intros.
+  repeat break_let.
+  unfold der_write_TL.
+  intros Z Z0 Z32 Zplus C.
+  erewrite Heqp.
+  erewrite Heqp0.
+  repeat break_if; try destruct_orb_hyp;
+  repeat Zbool_to_Prop; try rep_omega.
+  erewrite e in C.
+  congruence.
+  intuition.
+Qed.
+
+Definition Z_of_val v := 
+  match v with
+  | Vptr b i => Ptrofs.unsigned i 
+  | _ => 0
+  end.
+
+*)
+Definition Z_of_val v := 
+  match v with
+  | Vptr b i => Ptrofs.unsigned i 
+  | _ => 0
+  end.
